src/Reflection/MapCastByDeBruijnWf.v
@@ -9,8 +9,6 @@ Require Import Crypto.Reflection.Named.CompileWf.
 Require Import Crypto.Reflection.Named.PositiveContext.
 Require Import Crypto.Reflection.Named.PositiveContext.Defaults.
 Require Import Crypto.Reflection.Named.PositiveContext.DefaultsProperties.
-Require Import Crypto.Reflection.LinearizeWf.
-Require Import Crypto.Reflection.EtaWf.
 Require Import Crypto.Reflection.Syntax.
 Require Import Crypto.Reflection.MapCastByDeBruijn.
 Require Import Crypto.Util.Decidable.
@@ -76,12 +74,11 @@ Section language.
     : forall {b} e' (He':MapCast e input_bounds = Some (existT _ b e')),
       Wf e'.
   Proof.
-    unfold MapCastByDeBruijn.MapCast, MapCastCompile, MapCastDoCast, MapCastDoInterp, MapCastPreProcess, option_map; intros b e'.
+    unfold MapCastByDeBruijn.MapCast, MapCastCompile, MapCastDoCast, MapCastDoInterp, option_map; intros b e'.
     break_innermost_match; try congruence; intros ? v v'.
     inversion_option; inversion_sigma; subst; simpl in *; intros.
     unfold InterpretToPHOAS.Named.InterpToPHOAS, InterpretToPHOAS.Named.InterpToPHOAS_gen.
     destruct t as [src dst].
-    apply (proj2 (wf_expr_eta (t:=Arrow _ _))).
     eapply (@wf_interp_to_phoas
               base_type_code op FMapPositive.PositiveMap.key _ _ _ _
               (PositiveContext base_type_code _ base_type_code_beq base_type_code_bl_transparent)
@@ -90,9 +87,7 @@ Section language.
               (failb _) (failb _) _ e1);
       (eapply wf_map_cast with (fValues:=empty); eauto using PositiveContextOk with typeclass_instances);
       try (eapply (wf_compile (ContextOk:=PositiveContextOk));
-           [ eapply (proj2 (wf_expr_eta (t:=Arrow _ _)));
-             [ eapply wf_linearize | .. ];
-             eauto
+           [ eauto
            | ..
            | eassumption ]);
       try solve [ auto using name_list_unique_DefaultNamesFor
